bin_applications.v
@@ -1,0 +1,106 @@
+Require Import BinNat.
+Require Import Omega.
+Require Import micromega.Lia.
+Require Import Logic.FunctionalExtensionality.
+Require Import Nnat.
+Require Import bin_prelims.
+Require Import bin_repeater.
+Require Import bin_countdown.
+Require Import bin_inverse.
+
+Require applications.
+
+
+Fixpoint inv_hyperop (a : N) (n : nat) (b : N) :=
+  match n with
+  | 0%nat => b - 1
+  | 1%nat => b - a
+  | 2%nat => (b + a - 1) / a
+  | S n'  => countdown (inv_hyperop a n') 1 b
+  end.
+
+Theorem upp_inv_hyperop_0 : forall a,
+  upp_inv_rel (inv_hyperop a 0) (hyperop a 0).
+Proof. intros a b c. unfold hyperop. unfold inv_hyperop. lia. Qed.
+
+Theorem upp_inv_hyperop_1 : forall a,
+  upp_inv_rel (inv_hyperop a 1) (hyperop a 1).
+Proof. intros a b c. rewrite hyperop_1. unfold inv_hyperop. lia. Qed.
+
+Theorem upp_inv_hyperop_2 : forall a,
+  1 <= a -> upp_inv_rel (inv_hyperop a 2) (hyperop a 2).
+Proof.
+  intros a Ha b c. unfold inv_hyperop. rewrite hyperop_2.
+  repeat rewrite N.le_ngt. repeat rewrite <- N.le_succ_l.
+  rewrite le_div_mul by lia. repeat rewrite <- N.add_1_l. lia.
+Qed.
+
+Theorem inv_hyperop_0_correct : forall a b,
+  inv_hyperop a 0 b = N.of_nat (applications.inv_hyperop (N.to_nat a) 0 (N.to_nat b)).
+Proof. intros a b. simpl. lia. Qed.
+
+Theorem inv_hyperop_1_correct : forall a b,
+  inv_hyperop a 1 b = N.of_nat (applications.inv_hyperop (N.to_nat a) 1 (N.to_nat b)).
+Proof. intros a b. rewrite applications.inv_hyperop_1. simpl. lia. Qed.
+
+Theorem inv_hyperop_2_correct : forall a b, 1 <= a ->
+  inv_hyperop a 2 b = N.of_nat (applications.inv_hyperop (N.to_nat a) 2 (N.to_nat b)).
+Proof.
+  intros a b Ha. fold (applications.div (N.to_nat a) (N.to_nat b)).
+  apply le_antisym.
+  - rewrite (upp_inv_hyperop_2 a Ha _ b), hyperop_2, le_N_nat,
+     N2Nat.inj_mul, Nat2N.id, <- applications.div_correct by lia. trivial.
+  - rewrite le_N_nat, Nat2N.id, applications.div_correct, <- N2Nat.inj_mul,
+     <- le_N_nat, <- hyperop_2, <- (upp_inv_hyperop_2 a Ha _ b) by lia. lia.
+Qed.
+
+Lemma countdown_1_bin_contract_1 : forall f,
+    bin_contract_strict_above 1 f -> bin_contract_strict_above 1 (countdown f 1).
+Proof.
+  intros f Hf1. assert (H:=Hf1). destruct H as [Hf H1f].
+  split; intro n; [ |intro Hbn]; rewrite countdown_repeat by assumption;
+  rewrite N.le_ngt; intro; apply (repeat_bin_contract_strict _ _ _ _ Hf1) in H.
+  - specialize (nat_size_contract (n - 1)). rewrite N2Nat.inj_sub. omega.
+  - replace (nat_size (n - 1)) with (S (nat_size ((n - 1) / 2))) in H.
+    + assert (H0 := nat_size_contract ((n - 1) / 2)). simpl in H.
+      rewrite <- Nat.succ_le_mono in H. apply (Nat.le_trans _ _ _ H) in H0.
+      replace ((n + 1) / 2) with (1 + (n - 1) / 2) in H0. rewrite N2Nat.inj_add in H0.
+      simpl in H0. omega. rewrite <- N.div_add_l by lia. f_equal. lia.
+    + rewrite <- N.div2_div. destruct (n - 1); [simpl in H; omega|induction p; trivial].
+Qed.
+
+Lemma inv_hyperop_bin_contract : forall a n,
+    2 <= a -> (2 <= n)%nat -> bin_contract_strict_above 1 (inv_hyperop a n).
+Proof.
+  intros a n Ha Hn. destruct n as [|[|n]]; try omega. clear Hn. induction n.
+  - simpl. split; intro b; [destruct b|intro Hb];
+    rewrite N.le_ngt, <- N.le_succ_l, le_div_mul. 1,2,4,6: lia.
+    + remember (N.pos p - 1) as b. replace (N.succ _) with (N.succ b + 1) by lia.
+      replace (_ - 1) with (b + a) by lia. rewrite N.mul_add_distr_l, N.mul_1_r,
+      <- N.add_le_mono_r, <- N.lt_nge, <- N.le_succ_l, <- N.mul_1_l at 1.
+      apply N.mul_le_mono_r. lia.
+    + remember (b - 1) as c. replace (_ - 1) with (c + a * 1) by lia.
+      rewrite <- N.le_sub_le_add_r, <- N.mul_sub_distr_l.
+      replace (_ - 1) with (c / 2 + 1). intro.
+      assert (2 * (c/2 + 1) <= c) as contra.
+      { apply (N.le_trans _ (a * (c/2 + 1)) _); trivial.
+        apply N.mul_le_mono_r. apply Ha. }
+      rewrite <- le_div_mul in contra; lia. replace (_ - 1) with ((b + 1)/2) by lia.
+      replace (b + 1) with (c + 1 * 2) by lia. symmetry. apply N.div_add. lia.
+  - replace (inv_hyperop _ _) with (countdown (inv_hyperop a (S (S n))) 1) by trivial.
+    apply countdown_1_bin_contract_1. apply IHn.
+Qed.
+
+Theorem inv_hyperop_correct : forall a n,
+  2 <= a -> inv_hyperop a n = to_N_func (applications.inv_hyperop (N.to_nat a) n).
+Proof.
+  intros a n Ha. induction n as [|[|[|n]]].
+  1,2,3: apply functional_extensionality; intro b.
+  - apply inv_hyperop_0_correct.
+  - apply inv_hyperop_1_correct.
+  - apply inv_hyperop_2_correct. lia.
+  - replace (inv_hyperop _ _) with (countdown (inv_hyperop a (S (S n))) 1) by trivial.
+    apply (f_equal to_nat_func) in IHn. rewrite <- nat_N_func_id in IHn.
+    rewrite countdown_correct by (apply inv_hyperop_bin_contract; lia).
+    rewrite IHn. f_equal.
+Qed.
