old_bin_code/bin_applications.v
@@ -1,0 +1,25 @@
+Require Import BinNat.
+Require Import Omega.
+Require Import micromega.Lia.
+Require Import Logic.FunctionalExtensionality.
+Require Import Nnat.
+Require Import bin_prelims.
+Require Import bin_repeater.
+Require Import bin_countdown.
+Require Import bin_inverse.
+
+Require applications.
+
+Definition countdown_to_1 (f : N -> N) (n : N) : N
+  := countdown_worker f 1 n (nat_size (n - 1)).
+
+Theorem countdown_to_1 (f : N -> N) (n : N) : N
+  := 
+
+
+Fixpoint inv_hyperop (a : N) (n : nat) (b : N) :=
+  match n with
+  | 0%nat => b - 1
+  | 1%nat => b - a
+  | 2%nat => (b + a - 1) / a
+  | 
