old_bin_code/bin_inverse.v
@@ -1,0 +1,36 @@
+Require Import BinNat.
+Require Import Omega.
+Require Import micromega.Lia.
+Require Import Program.Basics.
+Require Import Nnat.
+Require Import bin_prelims.
+
+Require inverse.
+
+
+(* f is the upper inverse of F: f N is the smallest n such that F n >= N *)
+Definition upp_inv_rel (f F : N -> N) : Prop :=
+    forall n m, f m <= n <-> m <= F n.
+
+(* This version for N correctly mirrors its nat counterpart *)
+Theorem upp_inv_rel_correct : forall f F,
+    upp_inv_rel f F <-> inverse.upp_inv_rel (to_nat_func f) (to_nat_func F).
+Proof.
+  intros f F. unfold upp_inv_rel. unfold inverse.upp_inv_rel.
+  unfold to_nat_func. split; intros H n m.
+  - repeat rewrite le_nat_N. repeat rewrite N2Nat.id. apply H.
+  - specialize (H (N.to_nat n) (N.to_nat m)). repeat rewrite le_nat_N in H.
+    repeat rewrite N2Nat.id in H. apply H.
+Qed.
+
+(* Translation of the upper inverse computation from nat to N *)
+Definition upp_inv (F : N -> N) : N -> N := to_N_func (inverse.upp_inv (to_nat_func F)).
+
+Theorem upp_inv_correct :
+    forall F, increasing F -> upp_inv_rel (upp_inv F) F.
+Proof.
+  intros F HF n m. unfold upp_inv. unfold to_N_func.
+  rewrite le_N_nat, Nat2N.id. rewrite to_nat_func_incr in HF.
+  apply inverse.upp_inv_correct in HF. rewrite (HF _ _).
+  unfold to_nat_func. rewrite N2Nat.id. symmetry. apply le_N_nat.
+Qed.
