old_bin_code/bin_repeater.v
@@ -1,0 +1,166 @@
+Require Import BinNat.
+Require Import Program.Basics.
+Require Import Logic.FunctionalExtensionality.
+Require Import micromega.Lia.
+Require Import Nnat.
+Require Import Omega.
+Require Import bin_prelims.
+Require repeater.
+
+Open Scope N_scope.
+
+(*
+=============================================================================
+******* SECTION 2: HYPEROPS, ACKERMANN AND REPEATER *************************
+=============================================================================
+ *)
+
+(* We introduce "repeater" and how to use it to redefine the hyperoperations
+   and Ackermann function.
+   We also prove several results about the value of hypeopererations at small
+   numbers and levels, which are treated as known in the paper but need to be
+   rigourously proven here to be used in the proofs of theorems in the paper.
+   Several similar results for the Ackermann function are also provided.
+   Note that some results here may not be related to results in the paper, but
+   appear purely for aesthetics reasons. *)
+
+(* ****** REPEATER ********************************* *)
+
+Definition repeater (f : N -> N) (a : N) (n : N) : N :=
+  match n with
+  | 0      => a
+  | Npos p => let fix repeater_pos (g : N -> N) (p : positive) (a' : N) : N :=
+               match p with
+               | xH    => g a'
+               | xO p' => let g' := repeater_pos g p' in g' (g' a')
+               | xI p' => let g' := repeater_pos g p' in g (g' (g' a'))
+               end in repeater_pos f p a
+  end.
+
+(* Repeater is a functional way to look at repeat
+   See "repeat" in "prelims.v" *)
+Theorem repeater_repeat :
+    forall a f n, repeater f a n = repeat f (N.to_nat n) a.
+Proof.
+  intros a f n. destruct n; trivial. simpl.
+  generalize dependent a.
+  induction p; intro a; [ | |trivial];
+  [replace (Pos.to_nat p~1) with (S (Pos.to_nat p + Pos.to_nat p))%nat by lia|
+  replace (Pos.to_nat p~0) with (Pos.to_nat p + Pos.to_nat p)%nat by lia];
+    simpl; f_equal; rewrite repeat_plus; repeat rewrite IHp; trivial.
+Qed.
+
+(*
+(* Repeater on N is consistent with its counterpart on nat *)
+Theorem repeater_Nnat : 
+    forall a f, repeater f a =
+    to_N_func (repeater.repeater_from (to_nat_func f) (N.to_nat a)).
+Proof.
+  intros a f. apply functional_extensionality; intro n.
+  unfold to_N_func. rewrite repeater_repeat.
+  rewrite repeater.repeater_from_repeat.
+  remember (N.to_nat n) as m. clear Heqm. unfold to_nat_func.
+  induction m; simpl; [ |rewrite <- IHm]; rewrite N2Nat.id; trivial.
+Qed.
+*)
+
+(* Repeater on N is consistent with its counterpart on nat *)
+Theorem repeater_Nnat : 
+    forall a f n, repeater f a n =
+    N.of_nat (repeater.repeater_from (to_nat_func f) (N.to_nat a) (N.to_nat n)).
+Proof.
+  intros a f n. rewrite repeater_repeat.
+  rewrite repeater.repeater_from_repeat.
+  remember (N.to_nat n) as m. clear Heqm. unfold to_nat_func.
+  induction m; simpl; [ |rewrite <- IHm]; rewrite N2Nat.id; trivial.
+Qed.
+
+
+(* ****** HYPEROPS ********************************* *)
+
+(* A function to summarize the initial values of the hyperoperations *)
+Definition hyperop_init (a : N) (n : nat) : N :=
+  match n with 0%nat => a | 1%nat => 0 | _ => 1 end.
+
+(* Our definition for hyperops using repeater *)
+Fixpoint hyperop (a : N) (n : nat) (b : N) : N :=
+  match n with
+  | 0%nat => 1 + b
+  | S n'  => repeater (hyperop a n') (hyperop_init a n') b
+  end.
+
+(* A handy theorem to transform goals involving hyperops *)
+Lemma hyperop_recursion :
+  forall (n : nat) (a : N),
+    hyperop a (S n) = repeater (hyperop a n) (hyperop_init a n).
+Proof. intros. apply functional_extensionality. intro b. trivial. Qed.
+
+(* Proof that the two hyperops are the same *)
+Theorem hyperop_correct :
+  forall n a b, hyperop a n b = N.of_nat (repeater.hyperop (N.to_nat a) n (N.to_nat b)).
+Proof.
+  intros n a. induction n; intro b.
+  - unfold hyperop. unfold repeater.hyperop. lia.
+  - rewrite hyperop_recursion.
+    replace (repeater.hyperop (N.to_nat a) (S n) (N.to_nat b)) with
+    (repeater.repeater_from (repeater.hyperop (N.to_nat a) n)
+                          (repeater.hyperop_init (N.to_nat a) n)
+                          (N.to_nat b)) by trivial.
+    replace (repeater.hyperop_init (N.to_nat a) n) with
+    (N.to_nat (hyperop_init a n)) by repeat (destruct n; trivial).
+    rewrite repeater_Nnat. repeat f_equal.
+    apply functional_extensionality; intro c.
+    unfold to_nat_func. rewrite IHn. repeat rewrite Nat2N.id. trivial.
+Qed.
+
+(* The first few functions in the hyperops. Useful for pointing out
+   their inverse specifically *)
+
+Lemma hyperop_1 : forall a b, hyperop a 1 b = b + a.
+Proof.
+  intros. rewrite hyperop_correct. rewrite repeater.hyperop_1. lia.
+Qed.
+
+Lemma hyperop_2 : forall a b, hyperop a 2 b = b * a.
+Proof.
+  intros. rewrite hyperop_correct. rewrite repeater.hyperop_2. lia.
+Qed.
+
+Lemma hyperop_3 : forall a b, hyperop a 3 b = a ^ b.
+Proof.
+  intros. rewrite hyperop_correct. rewrite repeater.hyperop_3.
+  remember (N.to_nat a) as a0. replace a with (N.of_nat a0) by lia. clear Heqa0.
+  remember (N.to_nat b) as b0. replace b with (N.of_nat b0) by lia. clear Heqb0.
+  induction b0; trivial. replace (N.of_nat (S b0)) with (1 + N.of_nat b0) by lia.
+  rewrite N.pow_add_r. rewrite N.pow_1_r. simpl. rewrite <- IHb0. lia.
+Qed.
+
+(* A beautiful result about hypeops value at b = 1.
+   Used in the proof of the theorem "ack_hyperop",
+   which is also just for aesthetics *)
+Lemma hyperop_n_1 : forall n a, (2 <= n)%nat -> hyperop a n 1 = a.
+Proof.
+  intros n a Hn. do 2 (destruct n; [omega|]).
+  clear Hn. induction n; trivial.
+Qed.
+
+(* ****** ACKERMANN FUNCTION ********************************* *)
+
+(* Our definition using repeater *)
+Definition ackermann (n m : N) : N :=
+  let fix ack_nat (n0 : nat) (m0 : N) : N :=
+   match n0 with
+   | 0%nat => 1 + m0
+   | S n1  => repeater (ack_nat n1) (ack_nat n1 1) m0
+   end in ack_nat (N.to_nat n) m.
+
+(* Proof that the above are the same *)
+Theorem ackermann_correct : forall n m,
+  ackermann n m = N.of_nat (repeater.ackermann (N.to_nat n) (N.to_nat m)).
+Proof.
+  intros n m. unfold ackermann. unfold repeater.ackermann.
+  generalize dependent m. induction (N.to_nat n); intro m; [lia| ].
+  rewrite repeater_Nnat. repeat f_equal;
+  [unfold to_nat_func; apply functional_extensionality; intro p| ];
+  rewrite IHn0; repeat rewrite Nat2N.id; trivial.
+Qed.
